\documentclass[12pt]{article}
\usepackage[utf8]{inputenc}
\usepackage[russian]{babel}
\usepackage{parskip}

\begin{document}

\section*{S K K}

Дано: \\
S = $\lambda$x y z.x z (y z) \\
K = $\lambda$x y.x \\
I = $\lambda$x.x

Доказать: S K K = I

Доказательство:\\
($\lambda$x y z.x z (y z)) ($\lambda$x y.x) $\lambda$x y.x = (($\lambda$x y z.x z (y z)) ($\lambda$x y.x)) $\lambda$x y.x $\rightarrow_\beta$
($\lambda$y z.($\lambda$x y.x) z (y z)) $\lambda$x y.x
$\rightarrow_\beta$ \\
$\rightarrow_\beta$
($\lambda$y z.z) $\lambda$x y.x
$\rightarrow_\beta$
$\lambda$z.z

\section*{$\beta$-reduction}

(($\lambda$a.($\lambda$b.b b) ($\lambda$b.b b)) b) (($\lambda$c.(c b)) ($\lambda$a.a)) 
$\rightarrow_\beta$ \\
(($\lambda$b.b b) ($\lambda$b.b b)) (($\lambda$c.(c b)) ($\lambda$a.a)) 
$\rightarrow_\beta$ 
($\omega$ $\omega$) (($\lambda$c.(c b)) ($\lambda$a.a)) 
$\rightarrow_\beta$ \\
$\Omega$ (($\lambda$c.(c b)) ($\lambda$a.a)) 
$\rightarrow_\beta$ 
$\Omega$ (($\lambda$a.a) b)
$\rightarrow_\beta$ 
$\Omega$ b

\end{document}